Tweak rose trees defn, add induction principle from Steve

src/RoseTree.v
@@ -4,7 +4,12 @@
 (** printing rec %\coqdockw{rec}% *)
 (* begin hide *)
 From Equations Require Import Equations.
+
 Require Import Lia Utf8 List.
+
+From Coq Require Import
+     Arith.PeanoNat.
+
 Import ListNotations.
 Set Keyed Unification.
 
@@ -47,24 +52,42 @@ Obligation Tactic := CoreTactics.equations_simpl; try (simpl; lia); try typeclas
 (* begin hide *)
 Section RoseTree.
 (* end hide *)
-  Context {A : Type}.
+  (* Context {A : Type}. *)
 
   Inductive rose : Type :=
-    | leaf (a : A) : rose
-    | node (l : list rose) : rose.
+  | node (n : nat) (l : list rose) : rose.
 
   (** This is a nested inductive type we can measure assuming a
       [list_size] function for measuring lists. Here we use the usual
       guardedness check of %\Coq% that is able to unfold the
       definition of [list_size] to check that this definition is terminating. *)
 
-  Equations size (r : rose) : nat := size (leaf _) := 0; size (node l) := S (list_size size l).
+  Equations size (r : rose) : nat :=
+    size (node _ l) := S (list_size size l).
 
   (* begin hide *)
   Transparent size.
   Derive NoConfusion for rose.
 
   (* end hide *)
+  Section Induction.
+    Variable P : rose -> Prop.
+    Hypothesis IH_NODE : forall n children, (forall u, In u children -> P u) -> P (node n children).
+
+    Lemma rose_ind_strong : forall (t : rose), P t.
+    Proof.
+      fix IH 1.
+      destruct t.
+      apply IH_NODE.
+      revert l.
+      fix IHNODES 1. intros [|u children'].
+      - intros. inversion H.
+      - intros u' [<-|Hin].
+        + apply IH.
+        + eapply IHNODES. apply Hin.
+    Qed.
+  End Induction.
+
   (** As explained at the beginning of this section, however, if we want
       to program more complex recursions, or rearrange our terms
       slightly and freely perform dependent pattern-matching, the
@@ -74,24 +97,81 @@ Section RoseTree.
       well-founded recursion, we can define the following function
       gathering the elements in a rose tree efficiently: *)
 
-  Equations elements (r : rose) (acc : list A) : list A by wf (size r) lt :=
-  elements (leaf a) acc := a :: acc;
-  elements (node l) acc := aux l _
-    where aux x (H : list_size size x < size (node l)) : list A by wf (list_size size x) lt :=
+  Equations elements (r : rose) (acc : list rose) : list rose by wf (size r) lt :=
+  elements (node _ l) acc := aux l _
+    where aux x (H : list_size size x < size (node _ l)) : list rose by wf (list_size size x) lt :=
     aux nil _ := acc;
     aux (cons x xs) H := elements x (aux xs _).
 
   Definition elems r := elements r nil.
 
-  Equations parent (r1 : rose) (r2 : rose) : bool by wf (size r1) lt :=
-    parent (leaf a) (leaf b) := true;
-    parent _ _ := false.
-  parent (node l) (node l') := true.
-    where aux x (H : list_size size x < size (node l)) : list A by wf (list_size size x) lt :=
-    aux nil _ := acc;
-    aux (cons x xs) H := elements x (aux xs _).
+  Equations rose_eqb (r1 r2 : rose) : bool by wf (size r1) lt :=
+    rose_eqb (node n1 []) (node n2 []) := Nat.eqb n1 n2;
+    rose_eqb (node n1 (x :: xs)) (node n2 (y :: ys)) := rose_eqb (node n1 xs) (node n2 ys) && rose_eqb x y;
+    rose_eqb _ _ := false.
 
-  Definition elems r := elements r nil.
+  Lemma rose_eqb_refl : forall a, rose_eqb a a = true.
+  Proof.
+    induction a using rose_ind_strong.
+    induction children; simp rose_eqb.
+    - rewrite Nat.eqb_refl. reflexivity.
+    - rewrite IHchildren. rewrite H; auto.
+      + left. auto.
+      + intros. apply H. right. auto.
+  Qed.
+
+  Lemma rose_eqb_n : forall l l' n n', rose_eqb (node n l) (node n' l') = true -> n = n'.
+  Proof.
+    induction l; intros; simp rose_eqb in H; try inversion H.
+    2: {
+      destruct l'. inversion H.
+      simp rose_eqb in H. apply andb_prop in H. destruct H.
+      eapply IHl; eauto.
+    }
+    destruct l'. simp rose_eqb in H. apply EqNat.beq_nat_true in H. auto.
+    inversion H.
+  Qed.
+
+  Lemma rose_eqb_eq : forall a b, rose_eqb a b = true -> a = b.
+  Proof.
+    induction a using rose_ind_strong. induction children.
+    - intros. destruct b. destruct l. 2: inversion H0.
+      f_equal. apply rose_eqb_n in H0. auto.
+    - intros. destruct b. destruct l. inversion H0.
+      pose proof (rose_eqb_n _ _ _ _ H0). subst.
+      simp rose_eqb in H0. f_equal.
+      apply andb_prop in H0. destruct H0.
+      f_equal.
+      + apply H; auto. left. auto.
+      + epose proof (IHchildren _).
+        Unshelve.
+        2: { intros. apply H; auto. right. auto. }
+        specialize (H2 _ H0). inversion H2. auto.
+  Qed.
+
+  (* TODO *)
+  Axiom eq_rose : rose -> rose -> bool.
+  Axiom eq_rose_refl : forall a, eq_rose a a = true.
+  Axiom eq_rose_trans : forall a b c, eq_rose a b = true ->
+                                 eq_rose b c = true ->
+                                 eq_rose a c = true.
+
+  Equations parent (r1 : rose) (r2 : rose) : bool by wf (size r2) lt :=
+    parent a (node _ l) := match find (rose_eqb a) l with
+                           | Some _ => true
+                           | None => aux a l _
+                         end
+  where aux r1 (l' : list rose) (H : list_size size l' < size (node _ l)) : bool
+    by wf (list_size size l') lt :=
+    aux _ nil _ := false;
+    aux a' (cons x xs) H := parent a' x || aux a' xs _.
+
+  Goal parent (node 1 nil) (node 1 [node 1 [node 2 nil; node 1 nil]]) = true. auto. Qed.
+  Goal parent (node 1 nil) (node 1 [node 1 [node 2 nil; node 3 nil]]) = false. auto. Qed.
+  Goal parent (node 1 [node 2 nil; node 3 nil])
+       (node 1 [node 1 [node 2 nil; node 3 nil]]) = true. auto. Qed.
+  Goal parent (node 1 [node 2 nil])
+       (node 1 [node 1 [node 2 nil; node 3 nil]]) = false. auto. Qed.
 
   (**
     The function is nesting a well-founded recursion inside
@@ -112,9 +192,8 @@ Section RoseTree.
   (** We can show that [elems] is actually computing the same thing as
       the naïve algorithm concatenating elements of each tree in each forest. *)
 
-  Equations elements_spec (r : rose) : list A :=
-    elements_spec (leaf a) := [a];
-    elements_spec (node l) := concat (List.map elements_spec l).
+  Equations elements_spec (r : rose) : list rose :=
+    elements_spec (node _ l) := concat (List.map elements_spec l).
 
   (** As [elements] takes an accumulator, we first have to prove a generalized
       lemma, typical of tail-recursive functions: *)
@@ -122,7 +201,7 @@ Section RoseTree.
   Lemma elements_correct (r : rose) acc : elements r acc = elements_spec r ++ acc.
   Proof.
     apply (elements_elim (fun r acc f => f = elements_spec r ++ acc)
-             (fun l acc x H r => r = concat (List.map elements_spec x) ++ acc));
+                         (fun n l acc x H r => r = concat (List.map elements_spec x) ++ acc));
       intros; simp elements_spec; simpl; trivial. now rewrite H1, H0, app_assoc. Qed.
 
   (** We apply the eliminator providing the predicate for the nested
@@ -143,27 +222,3 @@ Section RoseTree.
 (* begin hide *)
 End RoseTree.
 (* end hide *)
-Arguments rose A : clear implicits.
-
-Module FullStruct.
-  Parameter (A : Type).
-
-  Equations elements (r : rose A) (acc : list A) : list A :=
-  elements (leaf a) acc := a :: acc;
-  elements (node l) acc := aux l
-    where aux (x : list (rose A)) : list A :=
-    aux nil := acc;
-    aux (cons x xs) := elements x (aux xs).
-End FullStruct.
-
-Module WfAndStruct.
-  Parameter (A : Type).
-
-  Equations elements (r : rose A) (acc : list A) : list A by wf (size r) lt :=
-  elements (leaf a) acc := a :: acc;
-  elements (node l) acc := aux l _
-    where aux (x : list (rose A)) (H : list_size size x < size (node l)) : list A by struct x :=
-    aux nil H := acc;
-    aux (cons x xs) H := elements x (aux xs _).
-
-End WfAndStruct.
